Normalize staged SimplifyCFG removal result

lowering/defs/evalCompilerBytecodeSimplifyCfgProbeScript.sml
@@ -59,4 +59,68 @@ Theorem exact_first_remove_unreachable:
 Proof
   ACCEPT_TAC first_remove_unreachable_th
 QED
+val first_removed_tm = rhs (concl first_remove_unreachable_th)
+Definition first_simplify_cfg_removed_def:
+  first_simplify_cfg_removed = ^first_removed_tm
+End
+
+Theorem exact_first_remove_unreachable_named:
+  remove_unreachable_blocks first_simplify_cfg_operand =
+    first_simplify_cfg_removed
+Proof
+  simp[first_simplify_cfg_removed_def, exact_first_remove_unreachable]
+QED
+
+Theorem first_simplify_cfg_dispatch_edge:
+  fn_succ first_simplify_cfg_operand "__entry" "@dispatch_1"
+Proof
+  simp[cfgTransformTheory.fn_succ_def,
+       venomInstTheory.lookup_block_def, venomInstTheory.bb_succs_def,
+       venomInstTheory.get_successors_def, venomInstTheory.is_terminator_def,
+       venomStateTheory.get_label_def, listTheory.FIND_def,
+       listTheory.INDEX_FIND_def, first_simplify_cfg_operand_def]
+QED
+
+Theorem first_simplify_cfg_fallback_edge:
+  fn_succ first_simplify_cfg_operand "__entry" "@fallback_0"
+Proof
+  simp[cfgTransformTheory.fn_succ_def,
+       venomInstTheory.lookup_block_def, venomInstTheory.bb_succs_def,
+       venomInstTheory.get_successors_def, venomInstTheory.is_terminator_def,
+       venomStateTheory.get_label_def, listTheory.FIND_def,
+       listTheory.INDEX_FIND_def, first_simplify_cfg_operand_def]
+QED
+
+val first_literal_edge_ths =
+  map (REWRITE_RULE [first_simplify_cfg_operand_def])
+    [first_simplify_cfg_dispatch_edge, first_simplify_cfg_fallback_edge]
+val first_removed_normal_th =
+  SIMP_CONV (srw_ss ()) first_literal_edge_ths first_removed_tm
+val first_removed_eq_operand_th =
+  SIMP_RULE (srw_ss ()) [GSYM first_simplify_cfg_operand_def,
+    GSYM first_simplify_cfg_blocks_th]
+    (TRANS first_simplify_cfg_removed_def first_removed_normal_th)
+
+Theorem first_simplify_cfg_removed_eq_operand:
+  first_simplify_cfg_removed = first_simplify_cfg_operand
+Proof
+  once_rewrite_tac [first_removed_eq_operand_th] >>
+  simp[venomInstTheory.ir_function_component_equality]
+QED
+
+val first_removed_blocks_eq_operand_th =
+  CONV_RULE (DEPTH_CONV BETA_CONV)
+    (AP_TERM ``\fn : ir_function. fn.fn_blocks``
+      first_simplify_cfg_removed_eq_operand)
+val first_removed_blocks_th =
+  TRANS first_removed_blocks_eq_operand_th first_simplify_cfg_blocks_th
+val first_removed_blocks =
+  fst (listSyntax.dest_list (rhs (concl first_removed_blocks_th)))
+
+Theorem first_simplify_cfg_removed_blocks:
+  ^(concl first_removed_blocks_th)
+Proof
+  ACCEPT_TAC first_removed_blocks_th
+QED
+
 val _ = export_theory()
